thys/JinjaThreads/Execute/Round_Robin.thy
@@ -608,7 +608,7 @@ lemma round_robin_step_correct:
   assumes det: "\<alpha>.deterministic I"
   and invar: "round_robin_invar \<sigma> (dom (thr_\<alpha> (thr s)))" "state_invar s" "state_\<alpha> s \<in> I"
   shows
-  "Option.map (apsnd (apsnd round_robin_\<alpha>)) (round_robin_step n0 \<sigma> s t) = 
+  "map_option (apsnd (apsnd round_robin_\<alpha>)) (round_robin_step n0 \<sigma> s t) = 
    \<alpha>.round_robin_step n0 (round_robin_\<alpha> \<sigma>) (state_\<alpha> s) t" (is ?thesis1)
   and "case_option True (\<lambda>(t, taxm, \<sigma>). round_robin_invar \<sigma> (case taxm of None \<Rightarrow> dom (thr_\<alpha> (thr s)) | Some (ta, x', m') \<Rightarrow> dom (thr_\<alpha> (thr s)) \<union> {t. \<exists>x m. NewThread t x m \<in> set \<lbrace>ta\<rbrace>\<^bsub>t\<^esub>})) (round_robin_step n0 \<sigma> s t)"
   (is ?thesis2)
@@ -645,7 +645,7 @@ lemma round_robin_reschedule_correct:
   assumes det: "\<alpha>.deterministic I"
   and invar: "round_robin_invar (queue, n) (dom (thr_\<alpha> (thr s)))" "state_invar s" "state_\<alpha> s \<in> I"
   and t0: "t0 \<in> set (queue_\<alpha> queue)"
-  shows "Option.map (apsnd (apsnd round_robin_\<alpha>)) (round_robin_reschedule t0 queue n0 s) =
+  shows "map_option (apsnd (apsnd round_robin_\<alpha>)) (round_robin_reschedule t0 queue n0 s) =
      \<alpha>.round_robin_reschedule t0 (queue_\<alpha> queue) n0 (state_\<alpha> s)"
   and "case_option True (\<lambda>(t, taxm, \<sigma>). round_robin_invar \<sigma> (case taxm of None \<Rightarrow> dom (thr_\<alpha> (thr s)) | Some (ta, x', m') \<Rightarrow> dom (thr_\<alpha> (thr s)) \<union> {t. \<exists>x m. NewThread t x m \<in> set \<lbrace>ta\<rbrace>\<^bsub>t\<^esub>})) (round_robin_reschedule t0 queue n0 s)"
 using t0 invar
@@ -679,7 +679,7 @@ next
       have "round_robin_invar (queue_enqueue t queue', n0) (dom (thr_\<alpha> (thr s)))"
         by(auto simp add: queue.enqueue_correct queue.push_correct)
       ultimately 
-      have "Option.map (apsnd (apsnd round_robin_\<alpha>)) (round_robin_reschedule t0 (queue_enqueue t queue') n0 s) =
+      have "map_option (apsnd (apsnd round_robin_\<alpha>)) (round_robin_reschedule t0 (queue_enqueue t queue') n0 s) =
             \<alpha>.round_robin_reschedule t0 (queue_\<alpha> (queue_enqueue t queue')) n0 (state_\<alpha> s)"
         using `state_invar s` `state_\<alpha> s \<in> I` by(rule rotate.hyps)
       thus ?thesis using None \<alpha>None `t \<noteq> t0` invar' queue'
@@ -713,7 +713,7 @@ qed
 lemma round_robin_correct:
   assumes det: "\<alpha>.deterministic I"
   and invar: "round_robin_invar \<sigma> (dom (thr_\<alpha> (thr s)))" "state_invar s" "state_\<alpha> s \<in> I"
-  shows "Option.map (apsnd (apsnd round_robin_\<alpha>)) (round_robin n0 \<sigma> s) =
+  shows "map_option (apsnd (apsnd round_robin_\<alpha>)) (round_robin n0 \<sigma> s) =
          \<alpha>.round_robin n0 (round_robin_\<alpha> \<sigma>) (state_\<alpha> s)"
     (is ?thesis1)
   and "case_option True (\<lambda>(t, taxm, \<sigma>). round_robin_invar \<sigma> (case taxm of None \<Rightarrow> dom (thr_\<alpha> (thr s)) | Some (ta, x', m') \<Rightarrow> dom (thr_\<alpha> (thr s)) \<union> {t. \<exists>x m. NewThread t x m \<in> set \<lbrace>ta\<rbrace>\<^bsub>t\<^esub>})) (round_robin n0 \<sigma> s)"
